\documentclass{article}
\usepackage[utf8]{inputenc}
\usepackage[english]{babel}
\usepackage [autostyle, english = american]{csquotes}
\MakeOuterQuote{"}
\usepackage{graphicx}
\usepackage{enumerate}
\usepackage{float}
\graphicspath{ {} }
\usepackage{mathtools}
\usepackage{amsmath, amsthm, amssymb, amsfonts}
\usepackage{caption}
\usepackage{bm}
\usepackage{fancyhdr}
\pagestyle{fancy}
\fancyhf{}
\rhead{Ty Darnell}
\lhead{Homework 6}

% For derivatives
\newcommand{\deriv}[1]{\frac{\mathrm{d}}{\mathrm{d}x} (#1)}

% For partial derivatives
\newcommand{\pderiv}[2]{\frac{\partial #1}{\partial #2}}

% Integral dx
\newcommand{\dx}{\mathrm{d}x}
\newcommand{\cd}{\overset{d}{\to}}
\newcommand{\cp}{\overset{p}{\to}}
\newcommand{\B}{\beta}
\newcommand{\e}{\epsilon}
\newcommand{\limn}{\lim_{n\to \infty}}
\newcommand{\lm}{\lambda}
\newcommand{\sg}{\sigma}
\newcommand{\hb}{\hat{\beta}}
\newcommand{\sumn}{\sum_{i=1}^{n}}
\newcommand{\hth}{\hat{\theta}}
\newcommand{\lra}{\Leftrightarrow}
\newcommand{\dll}[1]{\dfrac{\partial\ell({#1})}{\partial{#1}}}
\newcommand{\prodn}{\prod_{i=1}^{n}}
\allowdisplaybreaks
\begin{document}
\begin{flushleft}

	\section*{Problem 1}
	
\begin{enumerate}[(a)]
	
	\item 
\begin{multline*}\\
E(X^2)=Var(X)+[E(X)]^2=\sigma^2+\mu^2=\sigma^2+0\\
E(X^2)=\sg^2\\
\text{Thus } E(X^2) \text{ is an unbiased estimator of } \sg^2\\
\end{multline*}

	\item 
\begin{multline*}\\
L(\sigma|x)= \dfrac{1}{\sqrt{2\pi}\sigma}\exp\left(\dfrac{-x^2}{2\sigma^2} \right)\\
\ell(\sigma|x)=(-1/2)\log(2\pi)-\log(\sigma)-\dfrac{x^2}{2\sigma^2}\\
\propto -\log(\sigma)-\dfrac{x^2}{2\sigma^2}\\
\dll{\sg}=\dfrac{-1}{\sigma}+\dfrac{x^2}{\sigma^3}=0\\
\sigma^2=x^2\\
\hat{\sigma}=\sqrt{x^2}=|x|\\
\dll{\sigma^2}=\dfrac{1}{\sigma^2}-\dfrac{3x^2}{\sg^4}\\
\dll{\sigma^2}(\hat{\sg})=\dfrac{1}{|x|^2}-\dfrac{3x^2}{|x|^4}=\dfrac{1}{x^2}-\dfrac{3}{x^2}=\dfrac{-2}{x^2}<0\\
\text{Therefore } \hat{\sg} \text{ is the MLE}\\
\end{multline*}

	\item 
\begin{multline*}\\
M_1=0 \quad M_2=\sigma^2\\
E(X^2)=\sigma^2=\dfrac{1}{n}\sum_{i=1}^{1} X_i^2=X^2\\
\sigma^2=X^2\\
\sqrt{\sg^2}=\sqrt{X^2}\\
\hat{\sg}=|X|\\
\end{multline*}

\end{enumerate}

	\section*{Problem 2}
\begin{enumerate}[(a)]
	
	\item 
\begin{multline*}\\
L(\theta=0|x)=\prodn 1=1 \quad 0<x_i<1\\
L(\theta=1|x)=\prodn (1/2)x_i^{-1/2}=(1/2)^n\prodn x_i^{-1/2} \quad 0<x_i<1\\
MLE=0 \text{ if }  L(\theta=0|x)\geq L(\theta=1|x) \\
\text{Which is the same as } 1\geq (1/2)^n\prodn x_i^{-1/2}\\
MLE=1 \text{ if } L(\theta=0|x)< L(\theta=1|x) \\
\text{Which is the same as } 1<(1/2)^n\prodn x_i^{-1/2}\\
\end{multline*}

	\item 
\begin{multline*}\\
\text{Given } n=10 \quad \sumn \log(x_i)=-10.7\\
L(1|x)=(1/2)^{10}\prod_{i=1}^{10} x_i^{-1/2}\\
=(1/2)^{10}\exp\left(\sum_{i=1}^{10}\log(x_i^{-1/2})\right) \text{ since } \prodn a_n=\exp\left(\sumn \log(a_n)\right)\\
=(1/2)^{10}\exp\left((-1/2)\sum_{i=1}^{10}\log(x_i)\right)\\
=(1/2)^{10}\exp[(-1/2)(-10.7)]\\
=\dfrac{1}{1024}e^{5.35}\approx.20567\\
L(1|x)\approx .20567 \quad 0<x_i<1\\
L(0|x)=1 \quad 0<x_i<1\\
\text{Since } 1>.20567 \text{ the MLE of } \theta=0\\
\end{multline*}

\end{enumerate}

	\section*{Problem 3}
	
\begin{enumerate}[(a)]
	\item 
\begin{multline*}\\
X_1,\dots,X_n \sim\\
P(X_i\leq x|\alpha,\B)=\begin{cases}
0  & x<0\\
(x/\B)^{\alpha}  & 0\leq x\leq\B\\
1  & x>\B
\end{cases}\\
\alpha,\B>0\\
L(\alpha,\B|x)=f(x|\theta)=\prodn \dfrac{\alpha}{\B^{\alpha}}(x_i)^{\alpha-1} \ I[0,\B](x_i)\\
=\left(\dfrac{\alpha}{\B^\alpha}\right)^n\left(\prodn x_i\right)^{\alpha-1} I(x_{(n)}<\B)I(x_{(1)}>0)\\
f(\bm{x}|\theta)=g(T(\bm{x})|\theta)h(\bm{x}) \text{ where}\\
h(\bm{x})= I(x_{(1)}>0)\\ g(T(\bm{x})|\theta)=\left(\dfrac{\alpha}{\B^\alpha}\right)^n\left(\prodn x_i\right)^{\alpha-1} I(x_{(n)}<\B)\\
T(\bm{x})=\prodn x_i, x_{(n)}\\
\text{Thus by the factorization theorem, } \prodn x_i, x_{(n)} \text{ are sufficient}\\
\end{multline*}
	
	\item 
\begin{multline*}\\
L(\alpha,\B|x)=\left(\dfrac{\alpha}{\B^\alpha}\right)^n\left(\prodn x_i\right)^{\alpha-1}\\
\text{Fixing } \alpha L(\alpha,\B|x)=0 \text{ if } \B<x_{(n)}\\
L(\alpha,\B|x) \text{ is a decreasing function of } \B \text{ if } \B\geq x_{(n)}\\
\text{Therefore } \hat{\B}=x_{(n)} \text{ is the MLE of } \B\\
\ell(\alpha,\B|x)=\log\left( \left(\dfrac{\alpha}{\B^\alpha}\right)^n\left(\prodn x_i\right)^{\alpha-1} \right)\\
=n\log\alpha-\alpha n \log(\B)+(\alpha-1)\sumn \log(x_i)\\
\dll{\alpha}=\dfrac{n}{\alpha}-n \log(\B)+\sumn \log(x_i)=0\\
\text{Plug in } \hat{\B}=x_{(n)}\\
\dfrac{n}{\alpha}=n \log(x_{(n)})-\sumn \log(x_i)\\
\hat{\alpha}=\dfrac{n}{n \log(x_{(n)})-\sumn \log(x_i)}\\
\hat{\alpha}=\left[\dfrac{n \log(x_{(n)})-\sumn \log(x_i)}{n}\right]^{-1}\\
\hat{\alpha}=\left[\dfrac{1}{n}\sumn (\log(x_{(n)})-\log(x_i))\right]^{-1}\\
\dll{\alpha^2}=\dfrac{n}{\alpha}-n \log(x_{(n)})+\sumn \log(x_i)\\
=\dfrac{-n}{\alpha^2}<0\\
\text{Thus } \hat{\alpha} \text{ is the MLE}\\
\end{multline*}

	\item 
\begin{multline*}\\
\hb_{MLE} =X_{(n)}=25\\
\sumn \log(x_i)=40.81287\\
\hat{\alpha}_{MLE}=\dfrac{13}{13\log(25)-40.81287}=12.59055\\
\end{multline*}
	
\end{enumerate}
\pagebreak
	\section*{Problem 4}
	
\begin{enumerate}[(a)]
	
	\item 	
\begin{multline*}\\
f_y(y)=\dfrac{1}{\lm}e^{-y/\lm} \quad f_z(z)=\dfrac{1}{\mu}e^{-z/\mu}\\
\text{Since } Y\perp Z \text{ we can solve for the MLE individually}\\
L(\lambda|x)=\prodn \dfrac{1}{\lambda}e^{-y_i/\lm}=(1/\lambda)^n e^{-(1/\lm)\sumn y_i}\\
\ell(\lm|x)=-n\log(\lm)-(1/\lm)\sumn y_i\\
\dll{\lm}=\dfrac{-n}{\lm}+\dfrac{1}{\lm^2}\sumn y_i=0\\
\dfrac{n}{\lm}=\dfrac{1}{\lm^2}\sumn y_i=0\\
\hat{\lm}=\dfrac{1}{n}\sumn y_i=\bar{Y}\\
\dll{\lm^2}(\hat{\lm})=\dfrac{n}{(\dfrac{1}{n}\sumn y_i)^2}+\dfrac{-2}{(\dfrac{1}{n}\sumn y_i)^3}\sumn y_i=\dfrac{n}{(\dfrac{1}{n}\sumn y_i)^2}+\dfrac{-2n}{(\dfrac{1}{n}\sumn y_i)^2}\\
=\dfrac{-n}{(\dfrac{1}{n}\sumn y_i)^2}<0\\
\text{Thus } \hat{\lm} \text{ is the MLE}\\
\text{Same for } \hat{\mu}_{MLE} \text{ thus:}\\
\hat{\lm}_{MLE}=\bar{Y}\quad \hat{\mu}_{MLE}=\bar{Z}\\
\end{multline*}

	\item 
\begin{multline*}\\
X_i=\min(Y_i,Z_i) \\
\delta_i=\begin{cases}
1\text{, if } X_i=Y_i\\
0\text{, if } X_i=Z_i
\end{cases}\\
f_{X,\delta}(x,\delta)=\left(\dfrac{1}{\lm}\right)^{\delta}\left(\dfrac{1}{\mu}\right)^{1-\delta}e^{-\left(\dfrac{1}{\lm}+\dfrac{1}{\mu}\right)x}\\
L(\lm,\mu|x,\delta)=\prodn \left(\dfrac{1}{\lm}\right)^{\delta_i}\left(\dfrac{1}{\mu}\right)^{1-\delta_i}e^{-\left(\dfrac{1}{\lm}+\dfrac{1}{\mu}\right)x_i}\\
=\left(\dfrac{1}{\lm}\right)^{\sumn\delta_i}\left(\dfrac{1}{\mu}\right)^{n-\sumn \delta_i}e^{-\left(\dfrac{1}{\lm}+\dfrac{1}{\mu}\right)\sumn x_i}\\
\ell(\lm,\mu|x,\delta)=-\sumn\delta_i \log(\lambda)-(n-\sumn \delta_i)\log(\mu)-\left(\dfrac{1}{\lm}+\dfrac{1}{\mu}\right)\sumn x_i\\
\pderiv{\ell(\lm,\mu)}{\lm}=-\dfrac{1}{\lm}\sumn\delta_i +\dfrac{1}{\lm^2} \sumn x_i=0\\
\dfrac{1}{\lm}\sumn\delta_i=\dfrac{1}{\lm^2} \sumn x_i\\
\hat{\lm}= \dfrac{\sumn x_i}{\sumn\delta_i}\\
\pderiv{\ell^2(\lm,\mu)}{\lm^2}(\hat{\lm})=\dfrac{1}{\left[\dfrac{\sumn x_i}{\sumn\delta_i}\right]^2}\sumn\delta_i +\dfrac{-2}{\left[\dfrac{\sumn x_i}{\sumn\delta_i}\right]^3} \sumn x_i\\
=\dfrac{\left(\sumn\delta_i\right)^3}{\left(\sumn x_i\right)^2}-2\dfrac{\left(\sumn\delta_i\right)^3}{\left(\sumn x_i\right)^2}=-\dfrac{\left(\sumn\delta_i\right)^3}{\left(\sumn x_i\right)^2}<0\\
\text{Thus } \hat{\lm} \text{ is the MLE}\\
\pderiv{\ell(\lm,\mu)}{\mu}=-(n-\sumn \delta_i)\dfrac{1}{\mu}+\dfrac{1}{\mu^2}\sumn x_i=0\\
(n-\sumn \delta_i)\dfrac{1}{\mu}=\dfrac{1}{\mu^2}\sumn x_i\\
\hat{\mu}=\dfrac{\sumn x_i}{n-\sumn \delta_i}\\
\pderiv{\ell^2(\lm,\mu)}{\mu^2}(\hat{\mu})=(n-\sumn \delta_i)\left(\dfrac{n-\sumn \delta_i}{\sumn x_i}\right)^2-2\left(\dfrac{n-\sumn \delta_i}{\sumn x_i}\right)^3\sumn x_i\\
=\dfrac{\left(n-\sumn \delta_i\right)^3}{\left(\sumn x_i\right)^2}-2\dfrac{\left(n-\sumn \delta_i\right)^3}{\left(\sumn x_i\right)^2}=-\dfrac{\left(n-\sumn \delta_i\right)^3}{\left(\sumn x_i\right)^2}<0\\
\text{Thus } \hat{\mu} \text{ is the MLE}\\
\end{multline*}

\end{enumerate}
\pagebreak
	\section*{Problem 5}
\begin{enumerate}[(a)]
	
	\item 
\begin{multline*}\\
X_1,\dots,X_n \sim N(\mu_1) \quad \mu \text{ unknown}\\
Y_1,\dots,Y_n \text{ where } Y_i=I(X_i>0)\\
Y_i=\begin{cases}
1 \text{ if } X_i>0\\
0 \text{ if } X_i<0\\
\end{cases}\\
Y_i\sim Ber(P(Y_i=1))\\
\text{Let } \tau=P(Y_i=1)=P(X_i>0)\\
Y_i\sim Ber(\tau)\\
L(\tau|y)=\prodn \tau^{y_i}(1-\tau)^{1-y_i}\\
\end{multline*}

	\item 
\begin{multline*}\\
L(\tau|y)=\prodn \tau^{y_i}(1-\tau)^{1-y_i}\\
=\tau^{\sumn y_i}(1-\tau)^{\sumn 1- y_i}\\
\ell(\tau|y)=\sumn y_i \log(\tau)+(\sumn (1-y_i))\log(1-\tau)\\
\dll{\tau}=\dfrac{\sumn y_i}{\tau}-\dfrac{\sumn (1-y_i)}{1-\tau}=0\\
\dfrac{\sumn y_i}{\tau}=\dfrac{\sumn (1-y_i)}{1-\tau}\\
\dfrac{1-\tau}{\tau}=\dfrac{\sumn(1-y_i)}{\sumn y_i}\\
\dfrac{1}{\tau}=\dfrac{\sumn(1-y_i)}{\sumn y_i}+1\\
\hat{\tau}=\dfrac{\sumn y_i}{\sumn(1-y_i)+\sumn y_i}\\
=\dfrac{\sumn y_i}{n-\sumn(y_i)+\sumn y_i}\\
\hat{\tau}=\dfrac{1}{n}\sumn{y_i}=\bar{Y}\\
\dll{\tau^2}=\dfrac{-\sumn y_i}{\tau^2}-\dfrac{n-\sumn y_i}{(1-\tau)^2}\\
\text{Plugging in } \hat{\tau}=\bar{y}\\
=-\left(\dfrac{n\bar{y}}{\bar{y}^2}+\dfrac{n(1-\bar{y})}{(1-\bar{y})^2} \right)\\
=-n\left(\dfrac{1}{\bar{y}}+\dfrac{1}{1-\bar{y}}\right)<0\\
\text{Since the term inside the parenthesis is positive because } \bar{y}\leq1\\
\text{Thus } \hat{\tau} \text{ is the MLE}\\
\end{multline*}

\item 
\begin{multline*}\\
\tau=P(Y_i=1)=P(X_i>0)\\
\tau=P\left(\dfrac{X_i-\mu}{\sqrt{1}}>\dfrac{0-\mu}{\sqrt{1}}\right)\sim N(0,1)\\
\tau=1-\Phi(-\mu)\\
\mu=-\Phi^{-1}(1-\tau)\\
\hat{\mu}_{MLE}=-\Phi^{-1}(1-\hat{\tau}_{MLE})=-\Phi^{-1}(1-\bar{Y})\\
\end{multline*}

\end{enumerate}


\end{flushleft}
\end{document}
