\documentclass{article}
\usepackage[utf8]{inputenc}
\usepackage[english]{babel}
\usepackage{graphicx}
\usepackage{enumerate}
\usepackage{float}
\graphicspath{ {} }
\usepackage{mathtools}
\usepackage{amsmath, amsthm, amssymb, amsfonts}
\usepackage{caption}
\usepackage{fancyhdr}
\pagestyle{fancy}
\fancyhf{}
\rhead{Ty Darnell}
\lhead{Homework 4}

% For derivatives
\newcommand{\deriv}[1]{\frac{\mathrm{d}}{\mathrm{d}x} (#1)}

% For partial derivatives
\newcommand{\pderiv}[2]{\frac{\partial}{\partial #1} (#2)}

% Integral dx
\newcommand{\dx}{\mathrm{d}x}

\newcommand{\cd}{\overset{d}{\to}}
\newcommand{\cp}{\overset{p}{\to}}
\allowdisplaybreaks
\begin{document}
\begin{flushleft}

	\section*{Problem 1}
	
\begin{multline*}\\
\text{Using the central limit theorem } \bar{X_1} \text{ and } \bar{X_2} \text{ are approximatley normally distributed }\\
\bar{X_1} \sim N(\mu,\sigma^2/n)\\
\bar{X_2} \sim N(\mu,\sigma^2/n)\\
\text{Since } \bar{X_1} \text{ and } \bar{X_2} \text{ are independent:}\\
\bar{X_1}-\bar{X_2}\sim N(\mu_1-\mu_2,\sigma^2_1+\sigma^2_2)\\
\bar{X_1}-\bar{X_2}\sim N(0,2\sigma^2/n)\\
\text{Let } Z=\dfrac{[\bar{X_1}-\bar{X_2}]\sqrt{n}}{\sqrt{2}\sigma}\\
Z \sim N(0,1)\\
\text{We want to find n such that:}\\
P(|\bar{X_1}-\bar{X_2}|<\sigma/5)\approx .99\\ 
P(|\bar{X_1}-\bar{X_2}|<\sigma/5)=P(-\sigma/5<\bar{X_1}-\bar{X_2}<\sigma/5)\\
=P(\dfrac{-\sqrt{n}\sigma}{5\sqrt{2}\sigma}<Z<\dfrac{\sqrt{n}\sigma}{5\sqrt{2}\sigma})\\
=P(\dfrac{-\sqrt{n}}{5\sqrt{2}}<Z<\dfrac{\sqrt{n}}{5\sqrt{2}})\\
.99\approx P(\dfrac{-\sqrt{n}}{5\sqrt{2}}<Z<\dfrac{\sqrt{n}}{5\sqrt{2}})\\
.99\approx P(Z<\dfrac{\sqrt{n}}{5\sqrt{2}})-P(Z>-\dfrac{\sqrt{n}}{5\sqrt{2}})\\
.99\approx P(Z<\dfrac{\sqrt{n}}{5\sqrt{2}})-(1-P(Z<\dfrac{\sqrt{n}}{5\sqrt{2}}))\\
.99\approx 2P(Z<\dfrac{\sqrt{n}}{5\sqrt{2}})-1\\
P(Z<\dfrac{\sqrt{n}}{5\sqrt{2}})\approx .995\\
qnorm(.995)=2.575829 \quad \text{(using R)}\\
2.575829=\dfrac{\sqrt{n}}{5\sqrt{2}}\\
n=[2.575829(5\sqrt{2})]^2=50*2.575829^2=331.7448\\
n=332\\
\end{multline*}

	\section*{Problem 2}
\begin{enumerate}[(a)]
	
	\item 
\begin{multline*}\\
\text{Given } X_n \overset{p}{\to} a\\
\forall \ \epsilon>0 \quad \lim_{n\to \infty} P[|X_n-a|> \epsilon]=0\\
\text{WTS: } Y_i=\sqrt{X_i} \text{ converges in probability}\\
\text{That is:} \lim_{n\to \infty}P(|\sqrt{X_n}-\sqrt{a}>\epsilon)=0\\
P(|\sqrt{X_n}-\sqrt{a}>\epsilon)
=P(|\sqrt{X_n}-\sqrt{a}||\sqrt{X_n}+\sqrt{a}|>\epsilon|\sqrt{X_n}+\sqrt{a}|)\\
=P(|X_n-a|> \epsilon|\sqrt{X_n}+\sqrt{a}|)\\
\leq P(|X_n-a|> \epsilon\sqrt{a})\\
P(|\sqrt{X_n}-\sqrt{a}>\epsilon)\leq P(|X_n-a|> \epsilon\sqrt{a})\\
\text{Since } \forall \ \epsilon>0 \quad \lim_{n\to \infty} P[|X_n-a|> \epsilon]=0\\
\text{and } \epsilon\leq \sqrt{a}\epsilon\\
\text{We have }\lim_{n \to \infty}P(|X_n-a|> \epsilon\sqrt{a})=0\\
\text{Which means }\lim_{n\to \infty} P(|\sqrt{X_n}-\sqrt{a}>\epsilon)\leq\lim_{n \to \infty}P(|X_n-a|> \epsilon\sqrt{a})=0\\
\text{Thus }\lim_{n\to \infty} P(|\sqrt{X_n}-\sqrt{a}>\epsilon)= 0\\
\text{Therefore } \sqrt{X_n} \overset{p}{\to} \sqrt{a}\\
\end{multline*}
\begin{multline*}
\text{WTS: } Y_i^{'}=a/X_i \text{ converges in probability}\\
\text{That is:} \lim_{n\to \infty}P(|a/X_n-1|\leq\epsilon)=1\\
P(|a/X_n-1|\leq\epsilon)=P(-\epsilon\leq a/X_n-1\leq \epsilon)\\
=P\left(\dfrac{1-\epsilon}{a}\leq 1/X_n\leq \dfrac{1+\epsilon}{a}\right)\\
=P\left(\dfrac{a}{1+\epsilon}\leq X_n\leq \dfrac{a}{1-\epsilon}\right)\\
=P\left(\dfrac{a+a\epsilon-a\epsilon}{1+\epsilon}\leq X_n\leq \dfrac{a-a\epsilon+a\epsilon}{1-\epsilon}\right)\\
=P\left(\dfrac{a(1+\epsilon)-a\epsilon}{1+\epsilon}\leq X_n\leq \dfrac{a(1-\epsilon)+a\epsilon}{1-\epsilon}\right)\\
=P\left(a-\dfrac{a\epsilon}{1+\epsilon}\leq X_n\leq a+\dfrac{a\epsilon}{1-\epsilon}\right)\\
\geq P\left(a-\dfrac{a\epsilon}{1+\epsilon}\leq X_n\leq a+\dfrac{a\epsilon}{1+\epsilon}\right) \text{ Since } a+\dfrac{a\epsilon}{1+\epsilon}<a+\dfrac{a\epsilon}{1-\epsilon}\\
=P\left(-\dfrac{a\epsilon}{1+\epsilon}\leq X_n-a\leq \dfrac{a\epsilon}{1+\epsilon}\right)\\
=P\left(|X_n-a|\leq \dfrac{a\epsilon}{1+\epsilon} \right)\\
P(|a/X_n-1|\leq\epsilon)\geq P\left(|X_n-a|\leq \dfrac{a\epsilon}{1+\epsilon} \right)\\
\text{Since } \lim_{n\to \infty}P\left(|X_n-a|\leq \epsilon \right)=1\\
\text{We have }\lim_{n\to \infty}P\left(|X_n-a|\leq \dfrac{a\epsilon}{1+\epsilon} \right)=1\\
\text{Therefore } \lim_{n\to \infty}P(|a/X_n-1|\leq\epsilon)=1\\
\text{Thus } a/X_n \overset{p}{\to} 1\\
\end{multline*}
	\item 
\begin{multline*}\\
\text{WTS: } \dfrac{\sigma}{S_n}\overset{p}{\to} 1\\
\text{Using the result from the first part of a:}\\
X_n\overset{p}{\to} a \text{ means that }
\sqrt{X_n}\overset{p}{\to} \sqrt{a}\\
S_n=\sqrt{S_n^2}\\
\sqrt{S_n^2}\overset{p}{\to} \sqrt{\sigma^2}\\
S_n\overset{p}{\to} \sigma\\
\text{Using the result from the second part of a:}\\
X_n\overset{p}{\to} a \text{ means that } a/X_n\overset{p}{\to} 1\\
\text{Since } S_n\overset{p}{\to} \sigma\\
\dfrac{\sigma}{S_n}\overset{p}{\to} 1\\
\end{multline*}

\end{enumerate}
\pagebreak
	\section*{Problem 3}
	
\begin{multline*}\\
f_Y(y)=\theta \gamma^{\theta} y^{-(\theta+1)}\quad 0<\gamma<y<\infty, \ 2<\theta<\infty\\
F_Y(y)=1-\left(\dfrac{\gamma}{y}\right)^{\theta}\\
f_{Y_{(1)}}(y)=n(\theta \gamma^{\theta} y^{-(\theta+1)})\left[1-\left(1-\left(\dfrac{\gamma}{y}\right)^{\theta}\right)\right]^{n-1}\\
f_{Y_{(1)}}(y)=n\theta\gamma^{\theta n}y^{-(\theta n+1)} \quad 0<\gamma<y<\infty, \ 2<\theta<\infty\\
EY_{(1)}=\int_{\gamma}^{\infty}y(n\theta\gamma^{\theta n}y^{-(\theta n+1)}) \ dy\\
=n\theta\gamma^{\theta n}\int_{\gamma}^{\infty}y^{-\theta n} \ dy\\
=n\theta\gamma^{\theta n}\bigg|_{\gamma}^{\infty}\dfrac{1}{-\theta n+1}y^{-\theta n+1}\\
=\dfrac{n\theta\gamma^{\theta n}}{-\theta n+1}(0-\gamma^{-\theta n +1})\\
EY_{(1)}=\dfrac{-n\theta\gamma}{-\theta n+1}\\
\lim_{n\to \infty}EY_{(1)}=\lim_{n\to \infty}\dfrac{-n\theta\gamma}{-\theta n+1}\\
=\lim_{n\to \infty}\dfrac{-\theta\gamma}{-\theta +1/n}\\
=\dfrac{-\theta\gamma}{-\theta+0}=\gamma\\
\lim_{n\to \infty}EY_{(1)}=\gamma\\
Var(Y_{(1)})=E(Y_{(1)}^2)-(EY_{(1)})^2\\
E(Y_{(1)}^2)=\int_{\gamma}^{\infty}y^2(n\theta\gamma^{\theta n}y^{-(\theta n+1)}) \ dy\\
=n\theta\gamma^{\theta n}\int_{\gamma}^{\infty}y^{-\theta n+1} \ dy\\
=n\theta\gamma^{\theta n}\bigg|_{\gamma}^{\infty}\dfrac{1}{-\theta n+2}y^{-\theta n+2}\\
=\dfrac{n\theta\gamma^{\theta n}}{-\theta n+2}(0-\gamma^{-\theta n +2})\\
E(Y_{(1)}^2)=\dfrac{-n\theta\gamma^2}{-\theta n+2}\\
\lim_{n\to \infty} Var(Y_{(1)})=\lim_{n\to \infty} E(Y_{(1)}^2)- \lim_{n\to \infty}(EY_{(1)})^2\\
\lim_{n\to \infty}E(Y_{(1)}^2)=\lim_{n\to \infty}\dfrac{-n\theta\gamma^2}{-\theta n+2}\\
=\lim_{n\to \infty}\dfrac{-\theta \gamma^2}{-\theta+(2/n)}\\
=\dfrac{-\theta \gamma^2}{-\theta+0}=\gamma^2\\
\lim_{n\to \infty} E(Y_{(1)}^2)=\gamma^2\\
\lim_{n\to \infty} E(Y_{(1)})^2=\lim_{n\to \infty}\left(\dfrac{-n\theta\gamma}{-\theta n+1}\right)^2\\
=\lim_{n\to \infty}\dfrac{n^2\theta^2\gamma^2}{\theta^2 n^2-2\theta^2n+1}\\
=\lim_{n\to \infty}\dfrac{\theta^2\gamma^2}{\theta^2 -2\theta^2(1/n)+1/n^2}\\
=\dfrac{\theta^2\gamma^2}{\theta^2-0+0}=\gamma^2\\
\lim_{n\to \infty} E(Y_{(1)})^2=\gamma^2\\
\lim_{n\to \infty} Var(Y_{(1)})=\gamma^2-\gamma^2=0\\
\text{Thus } Y_{(1)} \text{ is a consistent estimator of } \gamma\\
Y_{(1)}\overset{p}{\to}\gamma\\
\end{multline*}
	\section*{Problem 4}
	
\begin{enumerate}[(a)]
	
	\item 	
\begin{multline*}\\
X_1,\dots,X_n \text{are iid random variables } \sim Pois(\mu) \quad \mu>0\\
E(X_i)=\mu \\
\bar{X_n}=n^{-1}\sum_{i=1}^{n}X_i\\
\sqrt{n}(\bar{X_n}-EX_1)\overset{d}{\to} N(0,\sigma^2)\\
\text{Since the mean and the variance of poisson rv are equal:}\\
\sigma^2=\mu \quad \sigma=\sqrt{\mu}\\
\text{Since we have iid random variables, a finite mean and variance:}\\
\dfrac{\sqrt{n}(\bar{X_n}-\mu)}{\sqrt{\mu}}\overset{d}{\to}N(0,1)\\
\end{multline*}

	\item 
\begin{multline*}\\
T_n=\sqrt{n}(\bar{X_n}-\mu)\\
T_n\overset{d}{\to}N(0,\mu)\\
\text{asymptotic variance } =\mu\\
\end{multline*}

	\item 
\begin{multline*}\\
\text{Want to find } h(\bar{X_n}) \text{ such that } h(\bar{X_n}) T_n \overset{d}{\to} N(0,1)\\
T_n=\sqrt{n}(\bar{X_n}-\mu)\overset{d}{\to} N(0,\mu)\\
\dfrac{\sqrt{n}(\bar{X_n}-\mu)}{\sqrt{\mu}}\overset{d}{\to}N(0,1) \text{ (CLT)}\\
\text{Since Xs are iid, } EX_i=\mu \text{, variance is finite:}\\
\bar{X_n}\overset{p}{\to} \mu \text{ (WLLN)}\\
\dfrac{\sqrt{\mu}}{\sqrt{\bar{X_n}}}\overset{p}{\to}1\\
\dfrac{\sqrt{\mu}}{\sqrt{\bar{X_n}}}\dfrac{\sqrt{n}(\bar{X_n}-\mu)}{\sqrt{\mu}}\overset{d}{\to}N(0,1) \text{ (Slutsky's Thm)}\\
\dfrac{\sqrt{n}(\bar{X_n}-\mu)}{\sqrt{\bar{\bar{X_n}}}}\overset{d}{\to}N(0,1)\\
g(\bar{X_n})\overset{p}{\to}g(\mu)\\
g(x)=\dfrac{1}{\sqrt{x}}\\
h(\bar{X_n})=\dfrac{1}{\sqrt{\bar{X_n}}}\\
\end{multline*}

	\item 
\begin{multline*}\\
95\% \text{ CI for } \mu:\\
\text{Since }\dfrac{\bar{X}-\mu)}{\sqrt{\bar{X_n}}}\overset{d}{\to}N(0,1)\\
.95\approx P\left(-1.96 <\dfrac{\sqrt{n}(\bar{X}-\mu)}{\sqrt{\bar{X_n}}}<1.96\right)\\
=P\left(\bar{X}+\dfrac{1.96\sqrt{\bar{X_n}}}{\sqrt{n}}>\mu>\bar{X}-\dfrac{1.96\sqrt{\bar{X_n}}}{\sqrt{n}} \right)\\
=P\left(\bar{X}-\dfrac{1.96\sqrt{\bar{X_n}}}{\sqrt{n}}<\mu<\bar{X}+\dfrac{1.96\sqrt{\bar{X_n}}}{\sqrt{n}} \right)\\
\text{Since }\dfrac{\bar{X}-\mu)}{\sqrt{\mu}}\overset{d}{\to}N(0,1)\\
\approx P\left(-1.96<\dfrac{\bar{X}-\mu)}{\sqrt{\mu}}<1.96\right)\\
\end{multline*}

	\item 
\begin{multline*}\\
\sqrt{n}(g(\bar{X_n})-g(\mu))\overset{d}{\to}N(0,1)\\
\sqrt{n}(g(\bar{X_n})-g(\mu))\overset{d}{\to}N(0,[g^{'}(\mu)]^2\mu)\\
[g^{'}(\mu)]^2\mu=1\\
[g^{'}(\mu)]^2=\dfrac{1}{\mu}\\
g^{'}(\mu)=\dfrac{1}{\sqrt{\mu}}=\mu^{-1/2}\\
g(\mu)=2\mu^{1/2}\\
\end{multline*}

\end{enumerate}

	\section*{Problem 5}
\begin{enumerate}[(a)]
	
	\item 
\begin{multline*}\\
X_1,\dots,X_n \sim N(\mu,1)\\
U_n=\dfrac{1}{\sqrt{n}}\sum_{i=1}^{n}(X_i-\mu)\\
\text{Want to find limiting distribution for } U_n\\
\sqrt{n}(\bar{X_n}-\mu) \overset{d}{\to}N(0,1) \text{ (CLT)}\\
=\sqrt{n}\left(\left[1/n\sum_{i=1}^{n}X_i\right]-\mu\right)\\
=\dfrac{1}{\sqrt{n}}\left(\sum_{i=1}^{n}X_i\right)-\sqrt{n}\mu\\
=\dfrac{1}{\sqrt{n}}\left(\sum_{i=1}^{n}(X_i-\mu)\right)=U_n\\
\text{Thus } U_n \overset{d}{\to} N(0,1)\\
\end{multline*}

	\item 
\begin{multline*}\\
X_1,\dots,X_n\sim N(\mu,1)\\
Var(X_i)=1\\
V_n=\dfrac{1}{n}\sum_{i=1}^{n}(X_i-\mu)^2\\
\text{WTS: } V_n \overset{p}{\to}1\\
\dfrac{1}{n}\sum_{i=1}^{n}X_i\overset{p}{\to}E(X_1) \text{ (WLLN)}\\
\dfrac{1}{n}\sum_{i=1}^{n}X_i^2\overset{p}{\to}E(X_i^2)\\
\text{If } Y_i=X_i^2 \text{ then } \dfrac{1}{n}\sum_{i=1}^{n}Y_i \cp E(Y_i)=E(X_i^2) \\
\text{Let } Y_i=X_i-\mu\\
V_n=\dfrac{1}{n}\sum_{i=1}^{n}(X_i-\mu)^2=\dfrac{1}{n}\sum_{i=1}^{n}Y_i^2\overset{p}{\to}E(Y_i^2)=E[(X_1-\mu)^2]=Var(X_i)=1\\
V_n \cp 1\\
\end{multline*}

	\item 
\begin{multline*}\\
W_n=U_n/V_n\\
U_n\cd N(0,1)\\
V_n\cp 1\\
U_n/V_n \cd N(0,1)/1=N(0,1) \text{ (Slutsky's Thm)}\\
\end{multline*}

	\item 
\begin{multline*}\\
\sqrt{n}(\bar{X}^2-\mu^2)\cd ?\\
\bar{X}=n^{-1}\sum_{i=1}^{n}X_i\\
\sqrt{n}(\bar{X}-\mu) \cd N(0,1)\\
\sqrt{n}(g(\bar{X_n})-g(\mu))\cd N(0,[g^{'}(\mu)]^2\sigma^2)\\
g(\mu)=\mu^2\\
g^{'}(\mu)=2\mu\\
N(0,[g^{'}(\mu)]^2\sigma^2)=N(0,[2\mu]^2(1))=N(0,4\mu^2)\\
\sqrt{n}(\bar{X}^2-\mu^2)\cd N(0,4\mu^2)\\
\end{multline*}

	\item 
\begin{multline*}\\X_1,\dots,X_n \sim N(\mu,1)\\
\bar{X}\sim N(\mu,1/n)\\
\text{Exact } 95\% \text{ CI}\\
.95=P\left(-1.96\leq\dfrac{\bar{X}-\mu}{\sqrt{1/n}}\leq 1.96 \right)\\
=P\left(\bar{X}-1.96\dfrac{1}{\sqrt{n}}\leq \mu\leq \bar{X}+1.96\dfrac{1}{\sqrt{n}} \right)\\
.95=P\left(L^2\leq \mu^2 \leq U^2 \right)\\
=P\left( \left[ \bar{X}-1.96\dfrac{1}{\sqrt{n}}\right]^2\leq \mu^2 \leq \left[ \bar{X}+1.96\dfrac{1}{\sqrt{n}}\right]^2 \right)\\
\end{multline*}	
\end{enumerate}

\end{flushleft}
\end{document}
