\documentclass{article}
\usepackage[utf8]{inputenc}
\usepackage[english]{babel}
\usepackage{graphicx}
\usepackage{enumerate}
\usepackage{float}
\graphicspath{ {} }
\usepackage{mathtools}
\usepackage{amsmath, amsthm, amssymb, amsfonts}
\usepackage{caption}
\usepackage{fancyhdr}
\pagestyle{fancy}
\fancyhf{}
\rhead{Ty Darnell}
\lhead{2016 Midterm Practice}

% For derivatives
\newcommand{\deriv}[1]{\frac{\mathrm{d}}{\mathrm{d}x} (#1)}

% For partial derivatives
\newcommand{\pderiv}[2]{\frac{\partial}{\partial #1} (#2)}

% Integral dx
\newcommand{\dx}{\mathrm{d}x}
\newcommand{\cd}{\overset{d}{\to}}
\newcommand{\cp}{\overset{p}{\to}}
\newcommand{\B}{\beta}
\newcommand{\e}{\epsilon}
\newcommand{\limn}{\lim_{n\to \infty}}
\newcommand{\lm}{\lambda}
\allowdisplaybreaks
\begin{document}
\begin{flushleft}

	\section*{Problem 1}
	
\begin{enumerate}[(a)]
	
	\item 
\begin{multline*}\\
X_1,\dots,X_n \sim U(0,\theta)\\
f_X(x)=\dfrac{1}{\theta} \quad 0<\theta<\infty\\
X_{(1)},\dots, X_{(n)} \text{ are order statistics}\\
Y_i=\dfrac{X_{i}}{X_{i+1}} \text{ for } i=1,\dots,n-1\\ Y_n=X_{(n)}\\
Y_{1}=\dfrac{X_{(1)}}{X_{(2)}} \quad Y_{n-1}=\dfrac{X_{(n-1)}}{X_{(n)}}\\
Y_n=X_{(n)}\\
X_{(n)}=Y_n \quad X_{(n-1)}=Y_n Y_{n-1} \ \cdots \ X_1=Y_1Y_2\cdots Y_n\\
X_{(i)}=\prod_{j=i}^{n}Y_j\\
J=\begin{bmatrix}
\dfrac{dx_1}{dy_1} & \dots & \dfrac{dx_1}{dy_n}\\
\dfrac{dx_2}{dy_1} &\dots &\dots\\
\dots &\dots &\dots\\
\dfrac{dx_n}{dy_1} & \dots & \dfrac{dx_n}{dy_n}
\end{bmatrix}\\
=\begin{bmatrix}
y_2\cdots y_n & \dots & y_1\cdots y_{n-1}\\
0 & y_3\cdots y_n & y_2\cdots y_{n-1}\\
\dots & \dots & \dots\\
0 & \dots & 1
\end{bmatrix}\\
J \text{ is an upper triangular matrix thus its determinant is the product of its main diagonal}\\
J=|y_2 y_3^2 \dots y_n^{n-1}|=y_2 y_3^2 \dots y_n^{n-1}\\
\end{multline*}

	\item 
\begin{multline*}\\
f_{Y_1,\dots,Y_n}(y_1,\dots,y_n)=f_{X_{(1)},\dots,X_{(n)}}(\prod_{j=1}^{n}(y_j,\dots,y_n))|J|\\
=\dfrac{n!}{\theta^n}(y_2 y_3^2 \dots y_n^{n-1})\\
\text{This can be factored into functions of } y_i \text{ for } i=1,\dots,n\\
\text{Thus the } Ys \text{ are mutually independent}\\
\end{multline*}

	\item 
\begin{multline*}\\
\text{Since there is no } y_1 \text{ term:}\\
f_{Y_1}(y_1)=1 \quad 0<y_1<1\\
f_{Y_i}(y_i)=iy_i^{i-1} \quad 0<y_i<1\\
f_{Y_n}(y_n)=n\dfrac{y_n^{n-1}}{\theta^n}\\
F_{Y_n}(y_n)=\dfrac{y_n^n}{\theta^n} \quad 0<y<\theta\\
\text{Let } Z_n=Y_n/\theta\\
F_Z(z)=P(Z\leq z)=P(Y_n\leq Z\theta)=F_y(z\theta)\\
F_y(z\theta)=\dfrac{(z\theta)^n}{\theta^n}=z^n=F_Z(z)\\
f_Z(z)=nz^{n-1} \quad 0<z<1\\
Beta(n,1)= \dfrac{\Gamma(n+1)}{\Gamma(n)\Gamma(1)}z^{n-1}(1-z)^{1-1} \quad 0<z<1\\
=\dfrac{n!}{n-1!}z^{n-1}=nz^{n-1}\\
Z\sim Beta(n,1)\\
\end{multline*}

\end{enumerate}

	\section*{Problem 2}
\begin{enumerate}[(a)]
	
	\item 
\begin{multline*}\\
\bar{X}=\dfrac{1}{n}\sum_{i=1}^{n}X_i\\
\bar{Y}=\dfrac{1}{n}\sum_{i=1}^{n}Y_i\\
\text{Since } X_1,\dots,X_n \text{ and } Y_1,\dots,Y_n \text{ are random samples from } N(\mu,\sigma^2):\\
\bar{X}\sim N(\mu,\sigma^2/n)\quad  \bar{Y}\sim N(\mu,\sigma^2/n)\\
\bar{X}-\bar{Y} \sim N(\mu-\mu,\sigma^2/n+(-\sigma)^2/n)=N(0,2\sigma^2/n)\\
\end{multline*}

	\item 
\begin{multline*}\\
\text{WTS: } \limn P(|\bar{X}-\bar{Y} |>\sigma)=0\\
P(|\bar{X}-\bar{Y} |>\sigma)=1-P(|\bar{X}-\bar{Y} |\leq\sigma)\\
=1-P(-\sigma\leq \bar{X}-\bar{Y}\leq \sigma)\\
=1-P\left(\dfrac{-\sigma}{\sqrt{2}\sigma/\sqrt{n}}\leq \dfrac{\bar{X}-\bar{Y}}{\sqrt{2}\sigma/\sqrt{n}}\leq \dfrac{\sigma}{\sqrt{2}\sigma/\sqrt{n}}\right)\\
1-P\left(-\sqrt{n/2}\leq \dfrac{\bar{X}-\bar{Y}}{\sqrt{2}\sigma/\sqrt{n}}\leq \sqrt{n/2}\right)\\
=1-(\Phi(\sqrt{n/2})-\Phi(-\sqrt{n/2}))\\
=1-\Phi(\sqrt{n/2})+\Phi(-\sqrt{n/2}))\\
\limn 1-\Phi(\sqrt{n/2})+\Phi(-\sqrt{n/2})\\
\limn \Phi(\sqrt{n/2})=\Phi(\infty) = 1 \quad \limn \Phi(-\sqrt{n/2})=\Phi(-\infty)=0\\
=1-1+0=0\\
\text{Thus }\limn P(|\bar{X}-\bar{Y} |>\sigma) = 0\\
\end{multline*}

\end{enumerate}

	\section*{Problem 3}
	
\begin{enumerate}[(a)]
	\item 
\begin{multline*}\\
X_1\sim pois(\lambda_1) \quad X_2\sim pois(\lambda_2)\\
X_1 \bot X_2\\
\text{WTS: } X_1|X_1+X_2 \sim bin(n,p) \text{ where}\\
E(X_1|X_2+X_2=n)=\dfrac{n\lambda_1}{\lambda_1+\lambda_2}\\
p=\dfrac{\lambda_1}{\lambda_1+\lambda_2}\\
(X_1+X_2=n) \sim pois(n|\lm_1+\lm_2)\\
= \dfrac{e^{-(\lm_1+\lm_2)}(\lm_1+\lm_2)^n}{n!}\\
f_{X_1,X_2}(x_1,x_2)=\dfrac{e^{-(\lm_1+\lm_2)}\lm_1^{x_1}}{x_1!}\dfrac{\lm_2^{x_2}}{x_2!}\\
P(X_1=x|X_1+X_2=n)=\dfrac{P(X_1=x,X_1+X_2=n)}{P(X_1+X_2=n)}\\
=\dfrac{P(X_1=x)P(X_2=n-x)}{P(X_1+X_2=n)}\\
=\dfrac{e^{-(\lm_1+\lm_2)}\lm_1^x\lm_2^{n-x}}{x!(n-x)!}/\dfrac{(\lambda_1+\lm_2)^n e^{-(\lm_1+\lm_2)}}{n!}\\
={n\choose x}\dfrac{e^{-(\lm_1+\lm_2)}\lm_1^x\lm_2^{n-x}}{(\lambda_1+\lm_2)^n e^{-(\lm_1+\lm_2)}}\\
={n\choose x}\dfrac{\lm_1^x\lm_2^{n-x}}{(\lambda_1+\lm_2)^n}\\
={n\choose x}\dfrac{\lm_1^x\lm_2^{n-x}}{(\lambda_1+\lm_2)^n}\dfrac{(\lambda_1+\lm_2)^{n-x}}{(\lambda_1+\lm_2)^{n-x}}\\
={n\choose x}\left(\dfrac{\lm_2}{\lm_1+\lm_2}\right)^{n-x}\left(\dfrac{\lm_1}{\lm_1+\lm_2}\right)^x\\
\text{Which is } bin(n,\dfrac{\lambda_1}{\lm_1+\lm_2})\\
\text{Thus } E(X_1|X_2+X_2=n)=\dfrac{n\lambda_1}{\lambda_1+\lambda_2}\\
\end{multline*} 

	\item                         
\begin{multline*}\\ 
\text{WTS: whether } T(X)=\sum_{i=1}^{2}X_i=X_1+X_2 \text{ is an SS for }\lm_1\\ 
P(X=x,T(X)=t)=\dfrac{P(X=x,X_1+X_2=t)}{P(X_1+X_t}\\
=\dfrac{P(X_1=x,X_2=x_2)}{P(X_1+X_2=t)}\\
=\dfrac{\lm_1^{x_1}e^{-\lm_1}\lm_2^{x_2}e^{-\lm_2}}{x_1!x_2!}/\dfrac{(\lm_1+\lm_2)^t e^{-(\lm_1+\lm_2)}}{t!}\\
=\dfrac{t!}{x_1!x_2!}\dfrac{\lm_1^{x_1}\lm_2^{x_2}}{(\lm_1+\lm_2)^t}\\
\text{This includes } \lm_1\\
\text{Thus } (X_1+X_2) \text{ not } \bot \lm_1\\
X_1+X_2 \text{ not SS of } \lm_1\\
\end{multline*}                

\end{enumerate}

	\section*{Problem 4}
	
\begin{enumerate}[(a)]
	
	\item 	
\begin{multline*}\\
f_X(x)=\dfrac{x^{\B-1}e^{-x}}{\Gamma(\B)} \quad x>0, \quad \B>1\\
f_T(t|X=x)=\theta xe^{-\theta xt} \quad t>0, \quad \theta>0\\
f_T(t)=\int_{0}^{\infty}f_{T,X}(t,x) \ \dx\\
=\int_{0}^{\infty}f_{T}(t|X=x)f_X(x) \ \dx\\
=\int_{0}^{\infty}\theta xe^{-\theta xt}\dfrac{x^{\B-1}e^{-x}}{\Gamma(\B)} \ \dx\\
=\dfrac{\theta}{\Gamma(\B)}\int_{0}^{\infty} x^{\B}e^{-(\theta t+1)x} \ \dx\\
\text{Want to get integral in the form of } gamma(\B+1,1/(\theta t+1))\\
=\dfrac{\Gamma(\B+1)\theta}{\Gamma(\B)(\theta t+1)^{\B+1}}\int_{0}^{\infty}\dfrac{(\theta t+1)^{\B+1}}{\Gamma(\B+1)} x^{\B}e^{-(\theta t+1)x} \ \dx\\
=\dfrac{\Gamma(\B+1)\theta}{\Gamma(\B)(\theta t+1)^{\B+1}}\\
f_T(t)=\dfrac{\B\theta}{(\theta t+1)^{\B+1}}\\
\end{multline*}
	
	\item 
\begin{multline*}\\
\text{WTS: } E(T)=\dfrac{1}{\theta(\B-1)}\\
E(T)=E(E(T|X=x))\\
E(T|X=x)=1/(\theta X) \text{ giving us:}\\
=E(1/(\theta X))=\dfrac{1}{\theta}E(X^{-1})\\
E(X^{-1})=\int_{0}^{\infty} x^{-1}f_X(x)\ \dx\\
=\int_{0}^{\infty} \dfrac{x^{\B-2}e^{-x}}{\Gamma(\B)} \ \dx\\
=\dfrac{\Gamma(\B-1)}{\Gamma(\B)}\int_{0}^{\infty} \dfrac{x^{\B-2}e^{-x}}{\Gamma(\B-1)} \ \dx\\
=\dfrac{\Gamma(\B-1)}{\Gamma(\B)}\\
=\dfrac{(\B-2)!}{(\B-1)!}\\
E(T)=\dfrac{1}{\theta}E(X^{-1})=\dfrac{1}{\theta(\B-1)}\\
\end{multline*}

	\item 
\begin{multline*}\\
\text{Given } \B=2 \quad E(T)=\dfrac{1}{\theta(2-1)}=\dfrac{1}{\theta}\\
\text{and } \sqrt{n}(\hat{\theta}-\theta)\cd N(0,2\theta^2) \quad T_n=\hat{\theta}\\
\text{Using delta method: }
\sqrt{n}\{g(T_n)-g(\theta)\}\cd N(0,\{g^{'}(\theta)\}^2 \sigma^2)\\
g(\theta)=\dfrac{1}{\theta} \quad g^{'}(\theta)=-\theta^{-2}\\
\sqrt{n}(1/\hat{\theta}-1/\theta)\cd N(0,\theta^{-4}2\theta^2)=N(0,2\theta^{-2})\\
\sigma^2=2\theta^{-2}\\
\end{multline*}

\end{enumerate}

\end{flushleft}
\end{document}
