\documentclass{article}
\usepackage[utf8]{inputenc}
\usepackage[english]{babel}
\usepackage{graphicx}
\usepackage{enumerate}
\usepackage{float}
\graphicspath{ {} }
\usepackage{mathtools}
\usepackage{amsmath, amsthm, amssymb, amsfonts}
\usepackage{caption}
\usepackage{fancyhdr}
\pagestyle{fancy}
\fancyhf{}
\rhead{Ty Darnell}
\lhead{Homework 9}

% For derivatives
\newcommand{\deriv}[1]{\frac{\mathrm{d}}{\mathrm{d}x} (#1)}

% For partial derivatives
\newcommand{\pderiv}[2]{\frac{\partial}{\partial #1} (#2)}

% Integral dx
\newcommand{\dx}{\mathrm{d}x}
\begin{document}
\begin{flushleft}
\chead{Problems 1-3}
\section*{Problem 1}
\begin{align*}
\text{Starting with the pdf of } &gamma(\alpha,\beta) \text{ we have:}\\
f(x|\alpha,\beta)&=\dfrac{1}{\Gamma(\alpha)\beta^{\alpha}}x^{\alpha-1}e^{-x/\beta}\\
\text{Then: } EX^{\nu}&=\int_{0}^{\infty}x^{\nu}\dfrac{1}{\Gamma(\alpha)\beta^{\alpha}}x^{\alpha-1}e^{-x/\beta} \dx\\
&=\int_{0}^{\infty}\dfrac{x^{\nu+\alpha-1}e^{-x/\beta} }{\Gamma(\alpha)\beta^{\alpha}}\dx\\
&=\dfrac{1}{\Gamma(\alpha)\beta^{\alpha}}\int_{0}^{\infty}x^{\nu+\alpha-1}e^{-x/\beta} \dx\\
\text{Let } y&=-x/\beta\\
&=\dfrac{(-\beta)(-\beta^{\alpha+\nu-1})}{\Gamma(\alpha)\beta^{\alpha}}\int_{0}^{\infty}y^{\nu+\alpha-1}e^{y} \ dy\\
\text{Since } \Gamma(\alpha+\nu)&=\int_{0}^{\infty}y^{\nu+\alpha-1}e^{y} \ dy \text{ we have:}\\
&=\dfrac{\beta^{\nu+\alpha}\Gamma(\nu+\alpha)}{\Gamma(\alpha)\beta^{\alpha}}\\
&=\dfrac{\beta^{\nu}\Gamma(\nu+\alpha)}{\Gamma(\alpha)}
\end{align*}
\section*{Problem 2}
\begin{align*}
Y&\sim negbin(r,p)\\
\text{WTS:} \lim \limits_{p \to 0}&M_{pY}(t)=\left(\dfrac{1}{1-t}\right)^r \text{ (the gamma(r,1) mgf)}\\
M_Y(t)&=\left(\dfrac{p}{1-(1-p)e^t}\right)^r\\
\text{Since } M_{aX+b}(t)&=e^{bt}M_X(at)\\
M_{pY}(t)&=\left(\dfrac{p}{1-(1-p)e^{pt}}\right)^r\\
\text{Since the limit is in a }& 0/0 \text{ indeterminate form we will use L'Hospitals Rule}\\
\lim \limits_{p \to 0}\left(\dfrac{\dfrac{d}{dp}p}{\dfrac{d}{dp}1-(1-p)e^{pt}}\right)^r&=\lim \limits_{p \to 0}\left(\dfrac{1}{e^{pt}+pte^{pt}-te^{pt}}\right)^r\\
&= \left(\dfrac{1}{1-t}\right)^r\\
\text{Thus limiting p to 0, the mgf of } &p_Y \text{ converges to the mgf of the gamma distribution}
\end{align*}
\section*{Problem 3}
\begin{enumerate}[(a)]
\item 
$E(X)$
\begin{align*}
f(x)&=\dfrac{2}{\sqrt{2\pi}}e^{-x^2/2}\\
E(X)&=\dfrac{2}{\sqrt{2\pi}}\int_{0}^{\infty}xe^{-x^2/2} \dx\\
&=\dfrac{2}{\sqrt{2\pi}}\bigg|_{0}^{\infty}-e^{-x^2/2}\\
&=\dfrac{2}{\sqrt{2\pi}}(0--1)=\dfrac{2}{\sqrt{2\pi}}\\
E(X)&=\dfrac{2}{\sqrt{2\pi}}
\end{align*}
$Var(X)$
\begin{align*}
E(X^2)&=\dfrac{2}{\sqrt{2\pi}}\int_{0}^{\infty}x^2e^{-x^2/2} \dx=\dfrac{2}{\sqrt{2\pi}}\sqrt{\pi/2}\\
&=\dfrac{\sqrt{2}}{\sqrt{\pi}}\dfrac{\sqrt{\pi}}{\sqrt{2}}=1\\
Var(X)&=E(X^2)-E(X)^2=1^2-\left(\dfrac{2}{\sqrt{2\pi}}\right)^2\\
&=1-\dfrac{4}{2\pi}=1-\dfrac{2}{\pi}
\end{align*}
\item 
\begin{align*}
\text{Given } f(x)&=\dfrac{2}{\sqrt{2\pi}}e^{-x^2/2}\\
\text{Find } g(X)&=Y \text{ so that:}\\
f(y|\alpha,\beta)&=\dfrac{1}{\Gamma(\alpha)\beta^{\alpha}}y^{\alpha-1}e^{-y/\beta}\\
\text{looking at the core parts}&\text{ of the two pdfs, we have:}\\
f_x&=e^{-x^2/2} \quad f_y=(y)^{\alpha-1} e^{-y/\beta}\\
\text{We will use the transformation }& Y=X^2\\
g^{-1}(y)&=\sqrt{y} \quad dy=(1/2)y^{-1/2}\\
f_y(y)&=\dfrac{\sqrt{2}}{\sqrt{\pi}}e^{-(y^{1/2})^2/2}(1/2)y^{-1/2}\\
&=\dfrac{1}{\sqrt{2 \pi}}y^{-1/2}e^{-1/2y}\\
\text{Since } \Gamma(1/2)&=\sqrt{\pi} \text{ let } \alpha=1/2 \text{, giving us:}\\
gamma(1/2,\beta)&=\dfrac{1}{\sqrt{\pi}\beta^{1/2}}y^{-1/2}e^{-y/\beta}\\
\text{in order to match}&\text{ our transformation let } \beta=2\\
&=\dfrac{1}{\sqrt{2 \pi}}y^{-1/2}e^{-1/2y}\\
\text{Thus we need the transformation }& Y=X^2 \text{ so that } Y\sim gamma(1/2,2)
\end{align*}
\end{enumerate}
\pagebreak
\section*{Problem 4}
\chead{Problems 4-6}
\begin{align*}
\text{Given } h_T(t)&=\lim \limits_{\delta \to 0} P(t\leq T\leq t+\delta|T\geq t)/\delta \text{, T is a continuos r.v.}\\
\text{WTS: } h_T(t)&=\dfrac{f_T(t)}{1-F_T(t)}=-\dfrac{d}{dt}\log(1-F_T(t))\\
P(t\leq T\leq t+\delta|T\geq t)&=\dfrac{P(t\leq T\leq t+\delta)}{P(T\geq t)}\\
&=\dfrac{F_T(t+\delta)-F_T(t)}{1-F_T(t)}\\
\text{Thus } h_T(t)&=\lim \limits_{\delta \to 0} \dfrac{F_T(t+\delta)-F_T(t)}{(1-F_T(t))\delta}\\
&\text{From the definition of a derivative we know:}\\
F^{'}_T(t)&=f_T(t)=\lim \limits_{\delta \to 0} \dfrac{F_T(t+\delta)-F_T(t)}{\delta}\\
\text{Which means: }h_T(t)&=\dfrac{f_T(t)}{1-F_T(t)} \text{ and }\\
-\dfrac{d}{dt}log(1-F_T(t))&=-\left(\dfrac{-f_T(t)}{1-F_T(t)}\right)=\dfrac{f_T(t)}{1-F_T(t)}\\
\text{Thus } h_T(t)&=\dfrac{f_T(t)}{1-F_T(t)}=-\dfrac{d}{dt}\log(1-F_T(t))
\end{align*}
\section*{Problem 5}
\begin{enumerate}[(a)]
\item 
\begin{align*}
f_T(t)&=1/\beta e^{-t/\beta}\\
F_T(t)&=\int_{0}^{t}1/\beta e^{-x/\beta} \dx =1-e^{-t/\beta}\\
h_T(t)&=\dfrac{f_T(t)}{1-F_T(t)}=\dfrac{1/\beta e^{-t/\beta}}{1-(1-e^{-t/\beta})}=\dfrac{(1/\beta) e^{-t/\beta}}{e^{-t/\beta}}=1/\beta\\
\end{align*}
\item
\begin{align*}
f_T(t)&=\gamma/\beta t^{\gamma-1}e^{-t^\gamma/\beta}\\
F_T(t)&=1-e^{-t^\gamma/\beta}\\
h_T(t)&=\dfrac{\gamma/\beta t^{\gamma-1}e^{-t^\gamma/\beta}}{1-(1-e^{-t^\gamma/\beta})}=\dfrac{\gamma/\beta t^{\gamma-1}e^{-t^\gamma/\beta}}{e^{-t^\gamma/\beta}}=(\gamma/\beta) t^{\gamma-1}
\end{align*}
\item 
\begin{align*}
f_T(t)&=\dfrac{e^{-(t-\mu)/\beta}}{\beta(1+e^{-(t-\mu)/\beta})^2}\\
F_T(t)&=\dfrac{1}{1+e^{-(t-\mu)/\beta}}\\
h_T(t)&=\dfrac{\dfrac{e^{-(t-\mu)/\beta}}{\beta(1+e^{-(t-\mu)/\beta})^2}}{1-(\dfrac{1}{1+e^{-(t-\mu)/\beta}})}\\
&=\dfrac{\dfrac{e^{-(t-\mu)/\beta}}{\beta(1+e^{-(t-\mu)/\beta})^2}}{\dfrac{e^{-(t-\mu)/\beta}}{1+e^{-(t-\mu)/\beta}}}=\dfrac{1}{\beta(1+e^{-(t-\mu)/\beta})}=(1/\beta)F_T(t)
\end{align*}
\end{enumerate}
\section*{Problem 6}
\begin{enumerate}[(a)]
\item 
\begin{align*}
f_X(x)&=\dfrac{1}{b-a} \quad x\in [a,b]\\
\text{Let } &m,x,y \in [a,b]\\
\text{Then } f(m)&=f(x)=f(y)\\
\text{since }\dfrac{1}{b-a}&=\dfrac{1}{b-a}=\dfrac{1}{b-a}\\
\text{Which means if }& m\geq  x \geq y \text{ or } m\leq x \leq y\\
\text{Then }f(m)\geq& f(x) \geq f(y)\\
\text{Thus the pdf of } &U(a,b) \text{ is unimodal}
\end{align*}
\item
\begin{align*}
f_X(x)&=x^{\alpha-1}e^{-x/\beta} \text{ ignoring constants }\\
\dfrac{d}{dx}f_X(x)&=\dfrac{x^{\alpha-2} e^{-x/\beta}(\beta(\alpha-1)-x)}{\beta}=0\\
x&=\beta(\alpha-1)\\
\text{Since there is only one sign change, } &f_X(x) \text{ is unimodal with mode } \beta(\alpha-1)
\end{align*}
\item 
\begin{align*}
f_X(x)&=e^{\left[\dfrac{-(x-\mu)^2}{2\sigma^2}\right]} \text{ ignoring constants}\\
\dfrac{d}{dx}f_X(x)&=\dfrac{x-\mu}{\sigma^2}e^{-(x-\mu)^2/(2\sigma^2)}=0\\
x&=\mu\\
\text{Since there is only one sign change, } &f_X(x) \text{ is unimodal with mode } \mu
\end{align*}
\item
\begin{align*}
f_X(x)&=x^{\alpha-1}(1-x)^{\beta-1} \text{ ignoring constants}\\
\dfrac{d}{dx}&=(\alpha-1)x^{\alpha-2}(1-x)^{\beta-1}-(\beta-1)x^{\alpha-1}(1-x)^{\beta-2}\\
&=(1-x)^{\beta-2}x^{\alpha-2}((\alpha-1)-x(\alpha+\beta-2)=0\\
x&=\dfrac{\alpha-1}{\alpha+\beta-2}\\
\text{Since there} &\text{ is only one sign change, } f_X(x) \text{ is unimodal with mode } \dfrac{\alpha-1}{\alpha+\beta-2}
\end{align*}
\end{enumerate}
\pagebreak
\section*{Problem 7}
\chead{Problems 7-9}
\begin{enumerate}[(a)]
\item 
\begin{align*}
f(x|\eta)&=h(x)c^*(\eta)\exp\left(\sum_{j=1}^{k}\eta_jt_j(x)\right)\\
\pderiv{\eta}1&=\dfrac{\partial}{\partial_{\eta}}\int h(x)c^*(\eta)\exp\left(\sum_{j=1}^{k}\eta_jt_j(x)\right)\dx\\
0&=\int\dfrac{\partial}{\partial_{\eta}}h(x)c^*(\eta)\exp\left(\sum_{j=1}^{k}\eta_jt_j(x)\right)\dx\\
&=\int h(x)c^{'*}(\eta)\exp\left(\sum_{j=1}^{k}\eta_jt_j(x)\right)\dx+\int h(x)c^{*}(\eta)\exp\left(\sum_{j=1}^{k}\eta_jt_j(x)\right)\left(\sum_{j=1}^{k}\dfrac{\partial \eta_j(\eta)}{\partial \eta_j}t_j(x) \right)\dx\\
&=\int h(x)\left[\dfrac{\partial}{\partial_{\eta}}\log(c^{*}(\eta))\right]c^{*}(\eta)\exp\left(\sum_{j=1}^{k}\eta_jt_j(x)\right)\dx+ E\left(\sum_{j=1}^{k}\dfrac{\partial \eta_j(\eta)}{\partial \eta_j}t_j(x) \right)\\
0&=\left[\dfrac{\partial}{\partial_{\eta}}\log(c^{*}(\eta))\right]+E\left(\sum_{j=1}^{k}\dfrac{\partial \eta_j(\eta)}{\partial \eta_j}t_j(x) \right)\\
&E\left(\sum_{j=1}^{k}\dfrac{\partial \eta_j(\eta)}{\partial \eta_j}t_j(x) \right)=-\left[\dfrac{\partial}{\partial_{\eta}}\log(c^{*}(\eta))\right]\\
&E(t_j(X))=E\left(\sum_{j=1}^{k}\dfrac{\partial \eta_j(\eta)}{\partial \eta_j}t_j(x) \right)\\
&E(t_j(X))=-\left[\dfrac{\partial}{\partial_{\eta}}\log(c^{*}(\eta))\right]
\end{align*}
\item 
\begin{align*}
f_X(x|a,b)&=\dfrac{1}{\Gamma(a)b^a}x^{a-1}\left(\sum_{j=1}^{k}\eta_jt_j(x)\right)\\
&=x^{-1}I(x>0)\dfrac{1}{\Gamma(a)b^a}e^{a \log{x}+(-1/b)x}\\
&=h(x)\dfrac{(-\eta_2)^{\eta_1}}{\Gamma(\eta_1)}e^{\eta_1 \log{x}+\eta_2 x}\\
EX&=-\pderiv{\eta_2}{\log\left(\dfrac{(-\eta_2)^{\eta_1}}{\Gamma(\eta_1)}\right)}\\
&=-\pderiv{\eta_2}{\eta_1 \log(-\eta_2)-\log\Gamma(\eta_1)}\\
&=\dfrac{\eta_1}{(-\eta_2)}=ab\\
EX&=ab\\
Var(X)&=-\dfrac{\partial^2}{\partial_{\eta_2^2}}\log\left(\dfrac{(-\eta_2)^{\eta_1}}{\Gamma(\eta_1)}\right)\\
&=\pderiv{\eta_2}{\dfrac{\eta_1}{-\eta_2}}=\dfrac{\eta_1}{\eta_2^2}=ab^2\\
Var(x)&=ab^2
\end{align*}
\end{enumerate}
\section*{Problem 8}
\begin{enumerate}[(a)]
\item 
\begin{align*}
f(x|\theta,\theta)&=\dfrac{1}{\sqrt{2\pi\theta}}e^{\left[\dfrac{-(x-\theta)^2}{2\theta^2}\right]}\\
&=\dfrac{1}{\sqrt{2\pi\theta}}e^{-\theta/2+x-x^2/(2\theta)}\\
h(x)=e^x \ I_{-\infty<x<\infty}(x) \quad c(\theta)&=\dfrac{1}{\sqrt{2\pi\theta}} \quad w_1(\theta)=1/2\theta \quad t_1(x)=-x^2\\
\text{Since } \mu&=\sigma^2 \text{ the } \theta \text{ parameter vector lies on the nonnegative real line} \\
\end{align*}
\item 
\begin{align*}
f(x|\theta,a\theta^2)&=\dfrac{1}{\sqrt{2\pi a\theta^2}}e^{\left[\dfrac{-(x-\theta)^2}{2a\theta^2}\right]}\\
&=\dfrac{1}{\sqrt{2\pi a\theta^2}}e^{-x^2/(2a\theta^2)+x/(a\theta)-1/2a}\\
h(x)&=I_{-\infty<x<\infty}(x) \quad c(\theta)=\dfrac{1}{\sqrt{2\pi a\theta^2}}e^{-1/2a}\\
w_1&=1/(2a\theta^2)  \quad w_2=1/(a\theta) \quad t_1=-x^2 \quad t_2=x\\
\text{Since } \mu^2&=a\sigma^2 \text{ the } \theta \text{ parameter vector lies on a parabola}\\
\end{align*}
\item 
\begin{align*}
f(x|a,1/a)&=\dfrac{1}{\Gamma(a)(1/a)^a}x^{a-1}e^{-ax}\\
&=\dfrac{a^a}{\Gamma(a)}\dfrac{1 }{x}x^{a}e^{-ax}\\
h(x)&= \dfrac{1}{x} \ I_{0<x<\infty}(x) \quad c(a)=a^a/\Gamma(a)\\
w_1(a)&=a \quad w_2(a)=a \quad t_1(x)=\log(x) \quad t_2(x)=-x\\
\text{The } &\theta \text{ parameter vector lies on a line}\\
\end{align*}
\item 
\begin{align*}
f(x|\theta)&=Ce^{-(x-\theta)^4}\\
&=Ce^{-\theta^4+4\theta^3x-6\theta^2x^2+4\theta x^3-x^4}\\
h(x)&=Ce^{-x^4}I_{-\infty<x<\infty}(x) \quad c(\theta)=e^{-\theta^4}\\
w_1(\theta)&=\theta \quad w_2(\theta)=\theta^2 \quad w_3(\theta)=\theta^3\\
t_1(x)&=4x^3 \quad t_2(x)=-6x^2 \quad t_3(x)=4x\\
\text{The } &\theta \text{ parameter vector lies on a 3 dimensional spiral}\\
\end{align*}
\end{enumerate}
\section*{Problem 9}
\begin{align*}
P(Z\geq t)&=\dfrac{1}{\sqrt{2\pi}}\int_{t}^{\infty}e^{-x^2/2}\dx\\
P(|Z|\geq t)&=2P(Z\geq t)\\
&=\dfrac{2}{\sqrt{2\pi}}\int_{t}^{\infty}e^{-x^2/2}\dx\\
&=\sqrt{\dfrac{2}{\pi}}\int_{t}^{\infty}\dfrac{1+x^2}{1+x^2}e^{-x^2/2}\dx\\
&=\sqrt{\dfrac{2}{\pi}}\left[\int_{t}^{\infty}\dfrac{1}{1+x^2}e^{-x^2/2}\dx+\int_{t}^{\infty}\dfrac{x^2}{1+x^2}e^{-x^2/2}\dx\right]\\
\text{integrating the}&\text{ second term by parts where:}\\
 u=\dfrac{x}{1+x^2} \quad dv&=xe^{-x^2/2} \quad v=-e^{-x^2/2} \quad du=\dfrac{1-x^2}{(1+x^2)^2}\\
\int_{t}^{\infty}\dfrac{x^2}{1+x^2}e^{-x^2/2}\dx&=\dfrac{x}{1+x^2}(-e^{-x^2/2})\bigg|_{t}^{\infty}+\int_{t}^{\infty}\dfrac{1-x^2}{(1+x^2)^2}e^{-x^2/2}dx\\
&=\dfrac{t}{t+t^2}e^{-t^2/2}+\int_{t}^{\infty}\dfrac{1-x^2}{(1+x^2)^2}e^{-x^2/2}dx\\
P(|Z|\geq t)&=\sqrt{\dfrac{2}{\pi}}\left(\dfrac{t}{t+t^2}e^{-t^2/2}+\int_{t}^{\infty}\dfrac{1}{1+x^2}e^{-x^2/2}\dfrac{1-x^2}{(1+x^2)^2}e^{-x^2/2}dx\right)\\
&=\sqrt{\dfrac{2}{\pi}}\left(\dfrac{t}{t+t^2}e^{-t^2/2}+\int_{t}^{\infty}\dfrac{(1+x^2)+1-x^2}{(1+x^2)^2}e^{-x^2/2}dx\right)\\
&=\sqrt{\dfrac{2}{\pi}}\dfrac{t}{t+t^2}e^{-t^2/2}+\sqrt{\dfrac{2}{\pi}}\int_{t}^{\infty}\dfrac{2}{(1+x^2)^2}e^{-x^2/2}\dx\\
&\geq \sqrt{\dfrac{2}{\pi}}\dfrac{t}{t+t^2}e^{-t^2/2}\\
\text{Therefore } P(|Z|\geq t)&\geq \sqrt{\dfrac{2}{\pi}}\dfrac{t}{t+t^2}e^{-t^2/2}
\end{align*}
\end{flushleft}
\end{document}
